NTCB/Validator.v
@@ -38,17 +38,19 @@ Module ValidatorCode (Import I: INSTRUCTION).
 
   Function validate_n_byte (n: N) (addr: N)
     (valid_addresses to_be_checked_addresses: NSet) (ll: lazy_list byte)
-    {measure nat_of_N n}: option (NSet * NSet * lazy_list byte):=
+    {measure nat_of_N n}: res (NSet * NSet * lazy_list byte):=
     match n with
       (* we are done with the validation of this block *)
-      | N0 => Some (valid_addresses, to_be_checked_addresses, ll)
+      | N0 => OK (valid_addresses, to_be_checked_addresses, ll)
 
       | _ => (* the do notation is defined in DoOption.  *)
 
         (* we parse the instruction *)
         do (instr, size_instr, ll') <- parse_instruction addr ll;
         (* and the number of byte left to validate *)
-        do n' <- safe_minus n size_instr;
+        match safe_minus n size_instr with
+        | None => Err "Instruction overlaps 32 bytes boundary"
+        | Some n' =>
 
         let addr' := addr + size_instr in
         match classify_instruction instr with
@@ -68,21 +70,25 @@ Module ValidatorCode (Import I: INSTRUCTION).
           | Mask_instr reg1 w =>
             match word_eq_dec w proper_mask with
               | left _ =>
-                (* if we are masking with the right mask, we check the next instruction*)
+              (* if we are masking with the right mask,
+                 we check the next instruction*)
                 match n' with
-                  | N0 => Some (Nadd addr valid_addresses, to_be_checked_addresses, ll')
+                  | N0 => OK (Nadd addr valid_addresses, to_be_checked_addresses, ll')
                   | _ =>
                     do (instr', size_instr', ll'') <- parse_instruction addr' ll';
                     match classify_instruction instr' with
                       | Indirect_jump reg2 => (* an indirect jump *)
                         match register_eq_dec reg1 reg2 with
                           | left _ => (* the proper register *)
-                            do n'' <- safe_minus n' size_instr';
+                            match safe_minus n' size_instr' with
+                            | None => Err "Instruction overlaps 32 bytes boundary"
+                            | Some n'' =>
                             let addr'' := addr' + size_instr' in
                             validate_n_byte n'' addr''
                               (Nadd addr valid_addresses) to_be_checked_addresses ll''
+                            end
                           (* an indirect jump that was not properly masked *)
-                          | right _ => None
+                          | right _ => Err "The mask used before the jump is incorrect"
                         end
                       | _ =>
                         validate_n_byte n' addr'
@@ -107,8 +113,9 @@ Module ValidatorCode (Import I: INSTRUCTION).
             else
               validate_n_byte n' addr' (Nadd addr valid_addresses)
                 (Nadd dest_addr to_be_checked_addresses) ll'
-          | Invalid_instruction
-          | Indirect_jump _ => None
+          | Invalid_instruction => Err "Invalid instruction"
+          | Indirect_jump _ => Err "Not masked indirect jump"
+        end
         end
     end.
   Proof.
@@ -116,7 +123,7 @@ Module ValidatorCode (Import I: INSTRUCTION).
     intros;
     repeat
       match goal with
-        | H : parse_instruction _ _ = Some _ |- _ =>
+        | H : parse_instruction _ _ = OK _ |- _ =>
           apply size_instr_not_0 in H
       end;
     repeat
@@ -160,36 +167,70 @@ Module ValidatorCode (Import I: INSTRUCTION).
       | |- context[ validate_n_byte ?n ?a ?va ?tbca ?ll] =>
         fun_ind_validate_n_byte_with
           (validate_n_byte n a va tbca ll)
+      | H : context[ validate_n_byte ?n ?a ?va ?tbca ?ll] |- _ =>
+        fun_ind_validate_n_byte_with
+          (validate_n_byte n a va tbca ll)
     end.
+  (* to lib *)
+  Inductive _MARK_:Prop := MARK.
+
+  Ltac pose_mark :=
+    generalize MARK.
+
+  Ltac intros_until_mark :=
+    repeat
+      (match goal with
+         | H : _MARK_ |- _ => fail 1
+         | _ => idtac
+       end; intro);
+      (match goal with
+         | H : _MARK_ |- _ => clear H
+         | _ => idtac
+       end).
+
+  Ltac clean_post_fun_ind_validate :=
+    clean;
+    pose_mark;
+    repeat
+    match goal with
+      | H: parse_instruction _ _ = OK _ |- _ =>
+        let H' := fresh H "'" in
+        pose proof H as H'; revert H';
+        apply parse_instruction_drops in H; symmetry in H; apply ll_safe_drop_size in H
+    end;
+    repeat
+    match goal with
+      | H: safe_minus _ _ = Some _ |- _ =>
+        let H' := fresh H "'" in
+        pose proof H as H'; revert H';
+          apply safe_minus_correct in H
+    end; intros_until_mark; subst
+    .
+
 
   Require Import Memory.
   Lemma validate_n_byte_reduces_size_by_n:
     forall n addr valid_addresses to_be_checked_addresses ll
       valid_addresses' to_be_checked_addresses' ll',
       validate_n_byte n addr valid_addresses to_be_checked_addresses ll =
-      Some (valid_addresses', to_be_checked_addresses', ll') ->
+      OK (valid_addresses', to_be_checked_addresses', ll') ->
       ll_length ll = (nat_of_N n + ll_length ll')%nat.
   Proof.
     intros ? ? ? ? ? ?.
 
-    fun_ind_validate_n_byte;
-      intros; clean;
-        try (specialize (IHo _ _ H));
-        apply parse_instruction_drops in e0; symmetry in e0; apply ll_safe_drop_size in e0;
-        apply safe_minus_correct in e2; try omega'.
-    apply parse_instruction_drops in e6; symmetry in e6; apply ll_safe_drop_size in e6;
-    apply safe_minus_correct in e10; try omega'.
+    fun_ind_validate_n_byte; intros; clean;
+      try (specialize (IHr _ _ H)); clean_post_fun_ind_validate; try omega'.
   Qed.
 
 
   Function validate_ll_list (addr: N)
     (valid_addresses to_be_checked_addresses: NSet) (ll: lazy_list byte)
-    {measure ll_length ll}: option (NSet * NSet):=
+    {measure ll_length ll}: res (NSet * NSet):=
     (* to validate a list, we repeatedly validate 32 byte blocks *)
     do (valid_addresses', to_be_checked_addresses', ll') <-
       validate_n_byte 32 addr valid_addresses to_be_checked_addresses ll;
     match ll' with
-      | 〈〉 => Some (valid_addresses', to_be_checked_addresses')
+      | 〈〉 => OK (valid_addresses', to_be_checked_addresses')
       | _ =>
         validate_ll_list (addr + 32) valid_addresses' to_be_checked_addresses' ll'
     end.
@@ -200,13 +241,31 @@ Module ValidatorCode (Import I: INSTRUCTION).
     simpl in *. destruct l. omega.
   Qed.
 
+  Ltac fun_ind_validate_ll_with call :=
+    functional induction call;
+      [ fst_Case_tac "fun_ind_validate_ll 1"
+      | fst_Case_tac "fun_ind_validate_ll 2"
+      | fst_Case_tac "fun_ind_validate_ll 3"].
+
+  Ltac fun_ind_validate_ll :=
+    match goal with
+      | |- context[ validate_ll_list ?a ?va ?tbca ?ll] =>
+        fun_ind_validate_ll_with
+          (validate_ll_list a va tbca ll)
+      | H: context[ validate_ll_list ?a ?va ?tbca ?ll] |- _  =>
+        fun_ind_validate_ll_with
+          (validate_ll_list a va tbca ll)
+    end.
+
+
   Definition validate_program ll :=
     (* to validate the program, we finally check the addresses left
        (the forward jumps) *)
-    match validate_ll_list header_size Nempty Nempty ll with
-      | None => false
-      | Some (valid_addresses, to_be_checked_addresses) =>
-        is_Nincluded to_be_checked_addresses valid_addresses
-    end.
+    do (valid_addresses, to_be_checked_addresses) <-
+      validate_ll_list header_size Nempty Nempty ll;
+    if is_Nincluded to_be_checked_addresses valid_addresses then
+      OK tt
+    else
+      Err "Direct jump to an invalid address".
 End ValidatorCode.
 
